Started definition check

src/Instructions.v
@@ -41,12 +41,121 @@ Record E2InstrWf : Prop := {
   e2instr_inj : inj_dom (acts_set G ∩₁ set_compl is_init) e2instr;
   nrmwend_even_tick : forall instr,
     tick ↑ restr_rel (fun x => instr_id x = instr) (e2instr ↑ nrmw_ord)
-      ⊆ (fun x y => y = 2 + x);
+      ⊆ (fun x y => y = 2 + x)⁺;
   rmw_ticks : forall instr,
     tick ↑ restr_rel (fun x => instr_id x = instr) (e2instr ↑ rmw_ord)
-      ⊆ (fun x y => y = 1 + x);
+      ⊆ (fun x y => y = 1 + x)⁺;
 }.
 
 End MainDefs.
+
+Section SanityCheck.
+
+Variable G : execution.
+Variable e2prog : actid -> nat.
+
+Hypothesis WF : Wf G.
+Hypothesis WEAK_INJ : forall x y (EQ : e2prog x = e2prog y), tid x = tid y.
+
+Definition ext_sb_ord := restr_rel (set_compl is_init) ext_sb.
+
+Lemma ninit_ext_sb_before_fin e :
+  set_finite (dom_rel (ext_sb_ord ⨾ ⦗eq e⦘)).
+Proof using.
+  destruct e as [el | et en].
+  { arewrite (ext_sb_ord ⨾ ⦗eq (InitEvent el)⦘ ≡ ∅₂).
+    { split; [| basic_solver].
+      unfold ext_sb_ord. unfolder. ins. desf. }
+    rewrite dom_empty. apply set_finite_empty. }
+  unfold ext_sb_ord. unfolder.
+  exists (map (ThreadEvent et) (List.seq 0 en)).
+  intros [xl | xt xn] (y & (SB & DOM & CODOM) & EQ).
+  all: subst; ins; desf.
+  apply in_map_iff. exists xn; split; eauto.
+  now apply in_seq0_iff.
+Qed.
+
+Lemma ninit_sb_before_fin e :
+  set_finite (dom_rel (nrmw_ord G ⨾ ⦗eq e⦘)).
+Proof using WF.
+  apply set_finite_mori with (x := dom_rel (ext_sb_ord ⨾ ⦗eq e⦘)).
+  all: try now apply ninit_ext_sb_before_fin.
+  red. unfold nrmw_ord, ext_sb_ord.
+  apply dom_rel_mori, seq_mori; ins.
+  apply restr_rel_mori; ins.
+  unfold sb. basic_solver.
+Qed.
+
+Lemma count_nrmw e :
+  { N : nat |
+    set_size (
+      dom_rel (nrmw_ord G ⨾ ⦗eq e⦘) ∩₁
+      fun x => e2prog x = e2prog e
+    ) = NOnum N }.
+Proof using WF.
+  apply ClassicalEpsilon.constructive_indefinite_description.
+  eapply set_size_finite, set_finite_mori,
+         ninit_sb_before_fin with (e := e).
+  red. basic_solver.
+Qed.
+
+Lemma count_nrmw_inj instr :
+  inj_dom
+    (set_compl is_init ∩₁ fun x => e2prog x = instr)
+    (fun e => proj1_sig (count_nrmw e)).
+Proof using WF WEAK_INJ.
+  unfolder. intros x y [XINIT XPROG] [YNINIT YPROG] EQ.
+  destruct (count_nrmw x) as [XN XSZ],
+           (count_nrmw y) as [YN YSZ]; ins.
+  rewrite XPROG in XSZ. rewrite YPROG in YSZ.
+  rewrite <- YPROG in XPROG. apply WEAK_INJ in XPROG.
+  clear YPROG. rename XPROG into TIDS.
+  subst YN. rename XN into N.
+  (* Should be true. We will see *)
+  admit.
+Admitted.
+
+Lemma check_rmw e :
+  { o : option actid | forall a,
+     << RMW : rmw G a e >> <-> << EQ : o = Some a >> }.
+Proof using WF.
+  apply ClassicalEpsilon.constructive_indefinite_description.
+  destruct (classic (codom_rel (rmw G) e)) as [CDOM|NCDOM].
+  { destruct CDOM as (y & RMW). exists (Some y). intros a.
+    split; intros HREL; desf.
+    { red. f_equal. eapply wf_rmwff; eauto. }
+    red in HREL. desf. }
+  exists None. intros a. split; intros HREL; desf.
+  red in HREL. exfalso. apply NCDOM. red; eauto.
+Qed.
+
+Definition nrmw_enum e : instruction_id :=
+  {|
+    instr_id := e2prog e;
+    tick := 2 * proj1_sig (count_nrmw e);
+  |}.
+
+Definition all_enum e : instruction_id :=
+  match proj1_sig (check_rmw e) with
+  | None => nrmw_enum e
+  | Some a => {|
+      instr_id := instr_id (nrmw_enum a);
+      tick := 1 + tick (nrmw_enum a);
+    |}
+  end.
+
+Lemma e2instr_correct : E2InstrWf G all_enum.
+Proof using WF.
+  constructor; ins.
+  { unfolder. intros x y (INX & XINIT) (INY & YINIY) EQ.
+    unfold all_enum in EQ.
+    destruct (check_rmw x) as [ox XIFF],
+             (check_rmw y) as [oy YIFF]; ins.
+    destruct ox as [ax |], oy as [ay |].
+    { admit. }
+    all: admit. }
+Admitted.
+
+End SanityCheck.
 
 End I2Exec.
